James C - added constraints

isabelle/Chapter13_2_Typechecking.thy
@@ -2,28 +2,115 @@ theory Chapter13_2_Typechecking
 imports Chapter13_1_Language
 begin
 
-inductive types_from_pat :: "patn => type => type list => bool"
-where tpwld [simp]: "types_from_pat Wild t []"
-    | tpvar [simp]: "types_from_pat PVar t [t]"
-    | tptrv [simp]: "types_from_pat PTriv Unit []"
-    | tppar [simp]: "types_from_pat p1 t1 ts1 ==> types_from_pat p2 t2 ts2 ==> 
-          types_from_pat (PPair p1 p2) (Prod t1 t2) (ts1 @ ts2)"
-    | tpinl [simp]: "types_from_pat p t1 ts ==> types_from_pat (PInL p) (Sum t1 t2) ts"
-    | tpinr [simp]: "types_from_pat p t2 ts ==> types_from_pat (PInR p) (Sum t1 t2) ts"
+datatype constr = 
+  All
+| And constr constr
+| Nothing
+| Or constr constr
+| CInL type type constr
+| CInR type type constr
+| CTriv
+| CPair constr constr
 
-inductive_cases [elim!]: "types_from_pat Wild t ts"
-inductive_cases [elim!]: "types_from_pat PVar t ts"
-inductive_cases [elim!]: "types_from_pat PTriv t ts"
-inductive_cases [elim!]: "types_from_pat (PPair p1 p2) t ts"
-inductive_cases [elim!]: "types_from_pat (PInL p) t ts"
-inductive_cases [elim!]: "types_from_pat (PInR p) t ts"
+inductive typecheck_constr :: "constr => type => bool"
+where [simp]: "typecheck_constr All t"
+    | [simp]: "typecheck_constr c1 t ==> typecheck_constr c2 t ==> typecheck_constr (And c1 c2) t"
+    | [simp]: "typecheck_constr Nothing t"
+    | [simp]: "typecheck_constr c1 t ==> typecheck_constr c2 t ==> typecheck_constr (Or c1 c2) t"
+    | [simp]: "typecheck_constr c t1 ==> typecheck_constr (CInL t1 t2 c) (Sum t1 t2)"
+    | [simp]: "typecheck_constr c t2 ==> typecheck_constr (CInR t1 t2 c) (Sum t1 t2)"
+    | [simp]: "typecheck_constr CTriv Unit"
+    | [simp]: "typecheck_constr c1 t1 ==> typecheck_constr c2 t2 ==> typecheck_constr (CPair c1 c2) (Prod t1 t2)"
 
-lemma [simp]: "types_from_pat p t ts ==> length ts = vars_count p"
-by (induction p t ts rule: types_from_pat.induct, simp_all)
+inductive_cases [elim!]: "typecheck_constr All t"
+inductive_cases [elim!]: "typecheck_constr (And x y) t"
+inductive_cases [elim!]: "typecheck_constr Nothing t"
+inductive_cases [elim!]: "typecheck_constr (Or x y) t"
+inductive_cases [elim!]: "typecheck_constr (CInL x y z) t"
+inductive_cases [elim!]: "typecheck_constr (CInR x y z) t"
+inductive_cases [elim!]: "typecheck_constr CTriv t"
+inductive_cases [elim!]: "typecheck_constr (CPair x y) t"
+
+inductive de_morgan_dual :: "constr => constr => bool"
+where "de_morgan_dual All Nothing"
+    | "de_morgan_dual c1 c1' ==> de_morgan_dual c2 c2' ==> de_morgan_dual (And c1 c2) (Or c1' c2')"
+    | "de_morgan_dual Nothing All"
+    | "de_morgan_dual c1 c1' ==> de_morgan_dual c2 c2' ==> de_morgan_dual (Or c1 c2) (And c1' c2')"
+    | "de_morgan_dual c c' ==> de_morgan_dual (CInL t1 t2 c) (Or (CInL t1 t2 c') (CInR t1 t2 All))"
+    | "de_morgan_dual c c' ==> de_morgan_dual (CInR t1 t2 c) (Or (CInR t1 t2 c') (CInL t1 t2 All))"
+    | "de_morgan_dual CTriv Nothing"
+    | "de_morgan_dual c1 c1' ==> de_morgan_dual c2 c2' ==> 
+          de_morgan_dual (CPair c1 c2) (Or (CPair c1' c2) (Or (CPair c1 c2') (CPair c1' c2')))"
+
+inductive_cases [elim!]: "de_morgan_dual All t"
+inductive_cases [elim!]: "de_morgan_dual (And x y) t"
+inductive_cases [elim!]: "de_morgan_dual Nothing t"
+inductive_cases [elim!]: "de_morgan_dual (Or x y) t"
+inductive_cases [elim!]: "de_morgan_dual (CInL x y z) t"
+inductive_cases [elim!]: "de_morgan_dual (CInR x y z) t"
+inductive_cases [elim!]: "de_morgan_dual CTriv t"
+inductive_cases [elim!]: "de_morgan_dual (CPair x y) t"
+
+lemma [simp]: "typecheck_constr c t ==> de_morgan_dual c c' ==> typecheck_constr c' t"
+by simp
+sorry
+
+inductive satisfies :: "expr => constr => bool"
+where [simp]: "satisfies e All"
+    | [simp]: "satisfies e c1 ==> satisfies e c2 ==> satisfies e (And c1 c2)"
+    | [simp]: "satisfies e c1 ==> satisfies e (Or c1 c2)"
+    | [simp]: "satisfies e c2 ==> satisfies e (Or c1 c2)"
+    | [simp]: "satisfies e c ==> satisfies (InL t1 t2 e) (CInL t1 t2 c)"
+    | [simp]: "satisfies e c ==> satisfies (InR t1 t2 e) (CInR t1 t2 c)"
+    | [simp]: "satisfies Triv CTriv"
+    | [simp]: "satisfies e1 c1 ==> satisfies e2 c2 ==> satisfies (Pair e1 e2) (CPair c1 c2)"
+
+inductive_cases [elim!]: "satisfies e All"
+inductive_cases [elim!]: "satisfies e (And x y)"
+inductive_cases [elim!]: "satisfies e Nothing"
+inductive_cases [elim!]: "satisfies e (Or x y)"
+inductive_cases [elim!]: "satisfies e (CInL x y z)"
+inductive_cases [elim!]: "satisfies e (CInR x y z)"
+inductive_cases [elim!]: "satisfies e CTriv"
+inductive_cases [elim!]: "satisfies e (CPair x y)"
+
+lemma "de_morgan_dual c c' ==> satisfies e c' = (~ satisfies e c)"
+proof auto
+  assume "de_morgan_dual c c'"
+     and "satisfies e c"
+     and "satisfies e c'"
+  thus False apply (induction c c' rule: de_morgan_dual.induct) by simp sorry
+next
+  assume "de_morgan_dual c c'"
+     and "~ satisfies e c"
+  thus "satisfies e c'" apply (induction c c' rule: de_morgan_dual.induct) by simp sorry
+qed
+
+definition totally_satisfied :: "constr => bool"
+where "totally_satisfied c = (ALL v. satisfies v c)" (* TODO: not all, but ALL v : typecheck env v t *)
+
+inductive types_from_pat :: "patn => type => type list => constr => bool"
+where tpwld [simp]: "types_from_pat Wild t [] All"
+    | tpvar [simp]: "types_from_pat PVar t [t] All"
+    | tptrv [simp]: "types_from_pat PTriv Unit [] CTriv"
+    | tppar [simp]: "types_from_pat p1 t1 ts1 c1 ==> types_from_pat p2 t2 ts2 c2 ==> 
+          types_from_pat (PPair p1 p2) (Prod t1 t2) (ts1 @ ts2) (CPair c1 c2)"
+    | tpinl [simp]: "types_from_pat p t1 ts c ==> types_from_pat (PInL p) (Sum t1 t2) ts (CInL t1 t2 c)"
+    | tpinr [simp]: "types_from_pat p t2 ts c ==> types_from_pat (PInR p) (Sum t1 t2) ts (CInR t1 t2 c)"
+
+inductive_cases [elim!]: "types_from_pat Wild t ts c"
+inductive_cases [elim!]: "types_from_pat PVar t ts c"
+inductive_cases [elim!]: "types_from_pat PTriv t ts c"
+inductive_cases [elim!]: "types_from_pat (PPair p1 p2) t ts c"
+inductive_cases [elim!]: "types_from_pat (PInL p) t ts c"
+inductive_cases [elim!]: "types_from_pat (PInR p) t ts c"
+
+lemma [simp]: "types_from_pat p t ts c ==> length ts = vars_count p"
+by (induction p t ts c rule: types_from_pat.induct, simp_all)
 
 inductive typecheck :: "(nat, type) assoc => expr => type => bool"
-      and typecheck_rules :: "(nat, type) assoc => rule list => type => type => bool"
-      and typecheck_rule :: "(nat, type) assoc => rule => type => type => bool"
+      and typecheck_rules :: "(nat, type) assoc => rule list => type => type => constr => bool"
+      and typecheck_rule :: "(nat, type) assoc => rule => type => type => constr => bool"
 where tvar [simp]: "lookup env v = Some t ==> typecheck env (Var v) t"
     | tzer [simp]: "typecheck env Zero Nat"    
     | tsuc [simp]: "typecheck env n Nat ==> typecheck env (Succ n) Nat"
@@ -41,10 +128,10 @@ where tvar [simp]: "lookup env v = Some t ==> typecheck env (Var v) t"
     | tabt [simp]: "typecheck env e Void ==> typecheck env (Abort t e) t"
     | tinl [simp]: "typecheck env e t1 ==> typecheck env (InL t1 t2 e) (Sum t1 t2)"
     | tinr [simp]: "typecheck env e t2 ==> typecheck env (InR t1 t2 e) (Sum t1 t2)"
-    | tmch [simp]: "typecheck env e t1 ==> typecheck_rules env rs t1 t2 ==> typecheck env (Match e rs) t2" 
-    | tnil [simp]: "typecheck_rules env [] t1 t2"
-    | tcns [simp]: "typecheck_rule env r t1 t2 ==> typecheck_rules env rs t1 t2 ==> typecheck_rules env (r # rs) t1 t2"
-    | trul [simp]: "types_from_pat p t1 ts ==> typecheck (extend_env ts env) e t2 ==> typecheck_rule env (Rule p e) t1 t2"
+    | tmch [simp]: "typecheck env e t1 ==> typecheck_rules env rs t1 t2 c ==> totally_satisfied c ==> typecheck env (Match e rs) t2" 
+    | tnil [simp]: "typecheck_rules env [] t1 t2 Nothing"
+    | tcns [simp]: "typecheck_rule env r t1 t2 c ==> typecheck_rules env rs t1 t2 cs ==> typecheck_rules env (r # rs) t1 t2 (Or c cs)"
+    | trul [simp]: "types_from_pat p t1 ts c ==> typecheck (extend_env ts env) e t2 ==> typecheck_rule env (Rule p e) t1 t2 c"
 
 inductive_cases [elim!]: "typecheck e (Var x) t"
 inductive_cases [elim!]: "typecheck e Zero t"
@@ -61,14 +148,14 @@ inductive_cases [elim!]: "typecheck e (Abort x y) t"
 inductive_cases [elim!]: "typecheck e (InL x y z) t"
 inductive_cases [elim!]: "typecheck e (InR x y z) t"
 inductive_cases [elim!]: "typecheck e (Match x y) t"
-inductive_cases [elim!]: "typecheck_rules e [] t t'"
-inductive_cases [elim!]: "typecheck_rules e (r # rs) t t'"
-inductive_cases [elim!]: "typecheck_rule e (Rule x y) t t'"
+inductive_cases [elim!]: "typecheck_rules e [] t t' c"
+inductive_cases [elim!]: "typecheck_rules e (r # rs) t t' c"
+inductive_cases [elim!]: "typecheck_rule e (Rule x y) t t' c"
                         
 lemma [simp]: "typecheck env e t ==> typecheck (extend_at env n k) (incr_from n e) t"
-  and [simp]: "typecheck_rules env rs t1 t2 ==> typecheck_rules (extend_at env n k) (incr_from_rules n rs) t1 t2"
-  and [simp]: "typecheck_rule env r t1 t2 ==> typecheck_rule (extend_at env n k) (incr_from_rule n r) t1 t2"
-proof (induction env e t and env rs t1 t2 and env r t1 t2 arbitrary: n and n and n rule: typecheck_typecheck_rules_typecheck_rule.inducts)
+  and [simp]: "typecheck_rules env rs t1 t2 c ==> typecheck_rules (extend_at env n k) (incr_from_rules n rs) t1 t2 c"
+  and [simp]: "typecheck_rule env r t1 t2 c ==> typecheck_rule (extend_at env n k) (incr_from_rule n r) t1 t2 c"
+proof (induction env e t and env rs t1 t2 c and env r t1 t2 c arbitrary: n and n and n rule: typecheck_typecheck_rules_typecheck_rule.inducts)
 case (tvar env v t)
   thus ?case by (simp add: incr_def) (* TODO: remove incr_def? *)
 next case tzer
@@ -104,15 +191,16 @@ next case tinl
   thus ?case by simp
 next case tinr
   thus ?case by simp
-next case (tmch env e t1 rs t2)
+next case (tmch env e t1 rs t2 c)
   hence "typecheck (extend_at env n k) (incr_from n e) t1" by simp
-  moreover from tmch have "typecheck_rules (extend_at env n k) (incr_from_rules n rs) t1 t2" by simp
+  moreover from tmch have "typecheck_rules (extend_at env n k) (incr_from_rules n rs) t1 t2 c" by simp
+  moreover from tmch have "totally_satisfied c" by simp
   ultimately show ?case by simp
 next case tnil
   thus ?case by simp
 next case tcns
   thus ?case by simp
-next case (trul p t1 ts env e t2)
+next case (trul p t1 ts c env e t2)
   from trul have "vars_count p = length ts" by simp
   moreover from trul have "typecheck (extend_at (extend_env ts env) (n + vars_count p) k) (incr_from (n + vars_count p) e) t2" by simp
   ultimately have "typecheck (extend_env ts (extend_at env n k)) (incr_from (n + vars_count p) e) t2" by simp
@@ -123,9 +211,9 @@ lemma [simp]: "typecheck env e t ==> typecheck (extend_env ts env) (incr_by (len
 by (induction ts, simp_all)        
 
 lemma [simp]: "typecheck (extend_at env n k) e t ==> n ~: free_vars e ==> typecheck env (sub_from n e) t"
-  and [simp]: "typecheck_rules (extend_at env n k) rs t1 t2 ==> n ~: free_vars_rules rs ==> typecheck_rules env (sub_from_rules n rs) t1 t2"
-  and [simp]: "typecheck_rule (extend_at env n k) r t1 t2 ==> n ~: free_vars_rule r ==> typecheck_rule env (sub_from_rule n r) t1 t2"
-proof (induction "extend_at env n k" e t and "extend_at env n k" rs t1 t2 and "extend_at env n k" r t1 t2 
+  and [simp]: "typecheck_rules (extend_at env n k) rs t1 t2 c ==> n ~: free_vars_rules rs ==> typecheck_rules env (sub_from_rules n rs) t1 t2 c"
+  and [simp]: "typecheck_rule (extend_at env n k) r t1 t2 c ==> n ~: free_vars_rule r ==> typecheck_rule env (sub_from_rule n r) t1 t2 c"
+proof (induction "extend_at env n k" e t and "extend_at env n k" rs t1 t2 c and "extend_at env n k" r t1 t2 c
        arbitrary: env n and env n and env n rule: typecheck_typecheck_rules_typecheck_rule.inducts)
 case (tvar v t)
   thus ?case by (cases "v < n", simp, cases "v = n", simp_all)
@@ -161,23 +249,24 @@ next case tinl
   thus ?case by simp
 next case tinr
   thus ?case by simp
-next case (tmch e t1 rs t2)
-  hence "typecheck_rules env (sub_from_rules n rs) t1 t2" by simp 
+next case (tmch e t1 rs t2 c)
+  hence "typecheck_rules env (sub_from_rules n rs) t1 t2 c" by simp 
   moreover from tmch have "typecheck env (sub_from n e) t1" by simp
+  moreover from tmch have "totally_satisfied c" by simp
   ultimately show ?case by simp
 next case tnil
   thus ?case by simp
 next case tcns
   thus ?case by simp
-next case (trul p t1 ts e t2)
+next case (trul p t1 ts)
   have "extend_at (extend_env ts env) (n + length ts) k = extend_env ts (extend_at env n k)" by simp
   with trul show ?case by simp
 qed
 
 lemma [simp]: "typecheck (extend env x t2) e t1 ==> typecheck env eb t2 ==> typecheck env (subst e eb x) t1"
-  and [simp]: "typecheck_rules (extend env x t2) rs t1a t1b ==> typecheck env eb t2 ==> typecheck_rules env (subst_rules rs eb x) t1a t1b"
-  and [simp]: "typecheck_rule (extend env x t2) r t1a t1b ==> typecheck env eb t2 ==> typecheck_rule env (subst_rule r eb x) t1a t1b"
-proof (induction "extend env x t2" e t1 and "extend env x t2" rs t1a t1b and "extend env x t2" r t1a t1b 
+  and [simp]: "typecheck_rules (extend env x t2) rs t1a t1b c ==> typecheck env eb t2 ==> typecheck_rules env (subst_rules rs eb x) t1a t1b c"
+  and [simp]: "typecheck_rule (extend env x t2) r t1a t1b c ==> typecheck env eb t2 ==> typecheck_rule env (subst_rule r eb x) t1a t1b c"
+proof (induction "extend env x t2" e t1 and "extend env x t2" rs t1a t1b c and "extend env x t2" r t1a t1b c
        arbitrary: env eb x and env eb x and env eb x rule: typecheck_typecheck_rules_typecheck_rule.inducts)
 case tvar
   thus ?case by auto
@@ -211,9 +300,10 @@ next case tinl
   thus ?case by simp
 next case tinr
   thus ?case by simp
-next case (tmch e t1 rs t2)
+next case (tmch e t1 rs t2 c)
   hence "typecheck env (subst e eb x) t1" by simp
-  moreover from tmch have "typecheck_rules env (subst_rules rs eb x) t1 t2" by simp
+  moreover from tmch have "typecheck_rules env (subst_rules rs eb x) t1 t2 c" by simp
+  moreover from tmch have "totally_satisfied c" by simp
   ultimately show ?case by simp
 next case tnil
   thus ?case by simp
