isabelle/Chapter13_3_PatternMatching.thy
@@ -94,8 +94,8 @@ next case (mtchr s p e)
   thus ?case by simp 
 qed
 
-lemma [simp]: "types_from_pat p t ts ==> typecheck env e t ==> is_val e ==> (EX s. typecheck_subst env s ts & matches s p e) | no_match e p"
-proof (induction p t ts arbitrary: e rule: types_from_pat.induct)
+lemma [simp]: "types_from_pat p t ts c ==> typecheck env e t ==> is_val e ==> (EX s. typecheck_subst env s ts & matches s p e) | no_match e p"
+proof (induction p t ts c arbitrary: e rule: types_from_pat.induct)
 case tpwld
   have "typecheck_subst env [] [] & matches [] Wild e" by simp
   hence "EX s. typecheck_subst env s [] & matches s Wild e" by (rule exI)
@@ -109,7 +109,7 @@ next case tptrv
   hence "typecheck_subst env [] [] & matches [] PTriv e" by simp
   hence "EX s. typecheck_subst env s [] \<and> matches s PTriv e" by (rule exI)
   thus ?case by simp
-next case (tppar p1 t1 ts1 p2 t2 ts2)
+next case (tppar p1 t1 ts1 c p2 t2 ts2)
   hence "(EX e1 e2. e = Pair e1 e2 & typecheck env e1 t1 & typecheck env e2 t2 & is_val e1 & is_val e2)" by (simp add: canonical_prod)
   with tppar show ?case
   proof auto
@@ -136,7 +136,7 @@ next case (tppar p1 t1 ts1 p2 t2 ts2)
       thus "EX s. typecheck_subst env s (ts1 @ ts2) & matches s (PPair p1 p2) (Pair e1 e2)" by auto
     qed
   qed
-next case (tpinl p t1 ts t2)
+next case (tpinl p t1 ts c t2)
   from tpinl have "(EX e'. e = InL t1 t2 e' & is_val e' & typecheck env e' t1) | (EX e'. e = InR t1 t2 e' & is_val e' & typecheck env e' t2)" by (simp add: canonical_sum)
   with tpinl show ?case
   proof (cases "EX e'. e = InL t1 t2 e'", auto)
@@ -148,7 +148,7 @@ next case (tpinl p t1 ts t2)
     hence "EX s. typecheck_subst env s ts & matches s p e'" by auto
     thus "EX s. typecheck_subst env s ts & matches s (PInL p) (InL t1 t2 e')" by auto
   qed
-next case (tpinr p t2 ts t1)
+next case (tpinr p t2 ts c t1)
   from tpinr have "(EX e'. e = InL t1 t2 e' & is_val e' & typecheck env e' t1) | (EX e'. e = InR t1 t2 e' & is_val e' & typecheck env e' t2)" by (simp add: canonical_sum)
   with tpinr show ?case
   proof (cases "EX e'. e = InR t1 t2 e'", auto)
@@ -200,5 +200,5 @@ proof auto
   moreover hence "s = s'" by simp
   ultimately show "typecheck env (apply_subst s e2) t" by simp
 qed 
-
+ 
 end
